removing the duplication of specs from buffer and wrappers

ulib/LowStar.Buffer.fst
@@ -10,21 +10,20 @@ module Seq = FStar.Seq
 module HS = FStar.HyperStack
 module HST = FStar.HyperStack.ST
 
-let trivial_preorder (a:Type0) :srel a = fun _ _ -> True
+(*
+ * Wrapper over LowStar.Monotonic.Buffer, with trivial preorders
+ *   -- functions that take explicit preorder as arguments (e.g. sub etc.)
+ *   -- these include allocation functions also
+ *)
+private let trivial_preorder (a:Type0) :srel a = fun _ _ -> True
 
 type buffer (a:Type0) = mbuffer a (trivial_preorder a) (trivial_preorder a)
 
 let null (#a:Type0) :buffer a = mnull #a #(trivial_preorder a) #(trivial_preorder a)
 
-let gsub (#a:Type0) (b:buffer a) (i:U32.t) (len:U32.t)
-  :Ghost (buffer a) (requires (U32.v i + U32.v len <= length b)) (ensures (fun _ -> True))
-  = mgsub b i len (trivial_preorder a)
+unfold let gsub (#a:Type0) = mgsub #a #(trivial_preorder a) #(trivial_preorder a) (trivial_preorder a)
 
-let gsub_inj (#a:Type0) (b1 b2:buffer a) (i1 i2:U32.t) (len1 len2:U32.t)
-  :Lemma (requires (U32.v i1 + U32.v len1 <= length b1 /\ U32.v i2 + U32.v len2 <= length b2 /\
-		    gsub b1 i1 len1 === gsub b2 i2 len2))
-         (ensures (len1 == len2 /\ (b1 == b2 ==> i1 == i2) /\ ((i1 == i2 /\ length b1 == length b2) ==> b1 == b2)))
-  = mgsub_inj b1 b2 i1 i2 len1 len2 (trivial_preorder a) (trivial_preorder a)
+unfold let gsub_inj (#a:Type0) = mgsub_inj #a #(trivial_preorder a) #(trivial_preorder a) (trivial_preorder a) (trivial_preorder a)
 
 inline_for_extraction
 type pointer (a:Type0) = b:buffer a{length b == 1}
@@ -32,59 +31,21 @@ type pointer (a:Type0) = b:buffer a{length b == 1}
 inline_for_extraction
 type pointer_or_null (a:Type0) = b:buffer a{if g_is_null b then True else length b == 1}
 
-(*
- * TODO: these are good candidates for letting F* infer WP,
- *       since their specs are just copied from their Monotonic.Buffer counterparts
- *)
-let sub (#a:Type0) (b:buffer a) (i:U32.t) (len:U32.t)
-  :HST.Stack (buffer a)
-             (requires (fun h -> U32.v i + U32.v len <= length b /\ live h b))
-             (ensures  (fun h y h' -> h == h' /\ y == gsub b i len))
-  = msub b i len (trivial_preorder a)
+inline_for_extraction let sub (#a:Type0) = msub #a #(trivial_preorder a) #(trivial_preorder a) (trivial_preorder a)
 
-let offset (#a:Type0) (b:buffer a) (i:U32.t)
-  :HST.Stack (buffer a)
-             (requires (fun h -> U32.v i <= length b /\ live h b))
-             (ensures  (fun h y h' -> h == h' /\ y == gsub b i (U32.sub (len b) i)))
-  = moffset b i (trivial_preorder a)
+inline_for_extraction let offset (#a:Type0) = moffset #a #(trivial_preorder a) #(trivial_preorder a) (trivial_preorder a)
 
+unfold let lbuffer (a:Type0) (len:nat) = lmbuffer a (trivial_preorder a) (trivial_preorder a) len
 
-unfold let lbuffer (a:Type0) (len:nat)
-  = b:buffer a{length b == len /\ not (g_is_null b)}
+inline_for_extraction let gcmalloc (#a:Type0) = mgcmalloc #a #(trivial_preorder a)
 
-let gcmalloc (#a:Type0) (r:HS.rid) (init:a) (len:U32.t)
-  :HST.ST (b:lbuffer a (U32.v len){frameOf b == r /\ recallable b})
-          (requires (fun _       -> HST.is_eternal_region r /\ U32.v len > 0))
-          (ensures  (fun h0 b h1 -> alloc_post_mem_common b h0 h1 (Seq.create (U32.v len) init)))
-  = mgcmalloc r init len
+inline_for_extraction let malloc (#a:Type0) = mmalloc #a #(trivial_preorder a)
 
-let malloc (#a:Type0) (r:HS.rid) (init:a) (len:U32.t)
-  :HST.ST (b:lbuffer a (U32.v len){frameOf b == r /\ freeable b})
-          (requires (fun _       -> HST.is_eternal_region r /\ U32.v len > 0))
-          (ensures  (fun h0 b h1 -> alloc_post_mem_common b h0 h1 (Seq.create (U32.v len) init)))
-  = mmalloc r init len
+inline_for_extraction let alloca (#a:Type0) = malloca #a #(trivial_preorder a)
 
-let alloca (#a:Type0) (init:a) (len:U32.t)
-  :HST.StackInline (lbuffer a (U32.v len))
-                   (requires (fun _       -> U32.v len > 0))
-                   (ensures  (fun h0 b h1 -> alloc_post_mem_common b h0 h1 (Seq.create (U32.v len) init) /\
-		                          frameOf b == HS.get_tip h0))
-  = malloca init len
+inline_for_extraction let alloca_of_list (#a:Type0) = malloca_of_list #a #(trivial_preorder a)
 
-let alloca_of_list (#a:Type0) (init: list a)
-  :HST.StackInline (lbuffer a (normalize_term (List.Tot.length init)))
-                   (requires (fun _      -> alloca_of_list_pre init))
-                   (ensures (fun h0 b h1 -> alloc_post_mem_common b h0 h1 (Seq.seq_of_list init) /\
-		                         frameOf b == HS.get_tip h0))
-  = malloca_of_list init
-
-let gcmalloc_of_list (#a:Type0) (r:HS.rid) (init:list a)
-  :HST.ST (b:lbuffer a (normalize_term (List.Tot.length init)){
-    frameOf b == r /\ 
-    recallable b})
-          (requires (fun _       -> HST.is_eternal_region r /\ gcmalloc_of_list_pre init))
-          (ensures  (fun h0 b h1 -> alloc_post_mem_common b h0 h1 (Seq.seq_of_list init)))
-  = mgcmalloc_of_list r init
+inline_for_extraction let gcmalloc_of_list (#a:Type0) = mgcmalloc_of_list #a #(trivial_preorder a)
 
 module L = FStar.List.Tot
 
